proofs.v
@@ -1,5 +1,5 @@
 Require Import ssreflect.
-From mathcomp Require Import ssreflect.seq.
+From mathcomp Require Import ssreflect seq ssrnat.
 From istari Require Import source subst_src rules_src help trans.
 From istari Require Import Sigma Tactics
      Syntax Subst SimpSub Promote Hygiene
@@ -25,46 +25,69 @@ Lemma subseq_type: forall G w1 w2,
 Ltac simpsub1 :=
   unfold leq_t; unfold leqtp; unfold nattp; unfold preworld; unfold app3; unfold nzero; simpsub; simpl.
 
-Lemma tr_weakening_append: forall G1 G2 J,
+Lemma tr_weakening_append: forall (G1: context) G2 J,
       tr G1 J ->
-      tr (G2 ++ G1) (substj (sh (length G2)) J).
-  intros. induction G2.
-  simpl. simpsub. assumption.
-  rewrite - app_comm_cons.
-  rewrite - (app_nil_l (a:: G2 ++ G1)).
-  suffices: (substctx sh1 nil = nil).
-  move => Heq.
-  rewrite - (Heq False).
-  
-  apply (tr_weakening (G2 ++ G1)).
+      tr (G2 ++ G1) (substj (sh (size G2)) J).
+ intros. induction G2.
+ -  simpl. simpsub. assumption.
+  - destruct J as [J1 J2]; subst.
+  suffices: (tr (substctx sh1 [::] ++ cons a (G2 ++ G1))
+                (substj (under (length [::]) sh1)
+                        (substj (sh (size G2)) (deq J1 J2 t)))).
+  move => Hdone.
+  simpl in Hdone.
+  rewrite (size_ncons 1).
+  rewrite - plusE. 
+  unfold substj.
+  repeat rewrite subst_sh_shift.
+  repeat rewrite - shift_sum.
+  repeat rewrite subst_sh_shift in Hdone.
+  rewrite cat_cons.
+ apply (Hdone False). 
+ intros.
+ eapply tr_weakening.
+ auto.
+Qed.
 
 Theorem one: forall G D e T ebar w1 l1,
     of_m G e T -> tr D (oof (ppair w1 l1) world) ->
     trans e ebar -> 
-         tr ((gamma_at G (ppair w1 l1)) ++ D) (oof (app ebar (subst (sh (length G)) l1))
+         tr ((gamma_at G w1 l1) ++ D) (oof (app ebar (subst (sh (length G)) l1))
                                                    (trans_type
                                                       (subst (sh (length G))
-                                                             (ppair w1 l1)) T) ).
+                                                             w1) (subst (sh (length G))
+                                                             l1)
+                                                    T )) .
   move => G D e T ebar w1 l1 Ds Dtrans.
   move : w1 l1 Dtrans. induction Ds; intros.
   10 : {
+    simpl.
+    eapply (tr_pi_elim _ nattp).
     inversion H; subst.
-    eapply tr_arrow_elim.
     eapply tr_pi_intro. eapply nat_type.
-    simpl. auto. simpsub.
     apply tr_all_intro.
     apply pw_kind.
-    auto. simpsub. simpl.
-    apply tr_pi_intro. simpsub. simpl.
-    unfold nattp. simpsub. apply nat_type.
+    rewrite subst_lam.
+    simpsub. simpl.
+    apply tr_pi_intro.  apply nat_type.
     eapply tr_eqtype_convert.
     eapply tr_eqtype_symmetry.
-    eapply tr_arrow_pi_equal. rewrite subseq_subst.
+    eapply tr_arrow_pi_equal.
     eapply tr_formation_weaken.
     apply subseq_type.
+    unfold world.
+    eapply tr_eqtype_convert.
+    eapply tr_eqtype_symmetry.
+      eapply tr_prod_sigma_equal.
+    eapply tr_formation_weaken; eapply tr_kuniv_weaken.
+    eapply pw_kind. eapply nat_type.
+    eapply tr_sigma_intro.
+    simpl.
+    rewrite subseq_subst.
     simpsub.
     induction G. simpsub.
     repeat rewrite compose_sh_dot.
+    auto.
     apply (tr_weakening D).
     apply tr_hyp_tm.
     try prove_subst.
